Lean4Axiomatic/Natural/Addition.lean
@@ -14,23 +14,28 @@ attribute [instance] Addition.Base.addOp
 class Addition.Derived (ℕ : Type) [Core ℕ] extends Addition.Base ℕ where
   add_zero {n : ℕ} : n + 0 ≃ n
   add_step {n m : ℕ} : n + step m ≃ step (n + m)
-  add_subst : AA.Substitutive₂ (α := ℕ) (· + ·) (· ≃ ·) (· ≃ ·)
+  add_substitutive : AA.Substitutive₂ (α := ℕ) (· + ·) (· ≃ ·) (· ≃ ·)
   add_one_step {n : ℕ} : n + 1 ≃ step n
-  add_comm : AA.Commutative (α := ℕ) (· + ·)
+  add_commutative : AA.Commutative (α := ℕ) (· + ·)
   add_assoc {n m k : ℕ} : (n + m) + k ≃ n + (m + k)
   cancel_add {n m k : ℕ} : n + m ≃ n + k → m ≃ k
   zero_sum_split {n m : ℕ} : n + m ≃ 0 → n ≃ 0 ∧ m ≃ 0
 
-attribute [instance] Addition.Derived.add_comm
-attribute [instance] Addition.Derived.add_subst
+attribute [instance] Addition.Derived.add_commutative
+attribute [instance] Addition.Derived.add_substitutive
 
 namespace Addition
 export Addition.Base (addOp step_add zero_add)
-export Addition.Derived
-  (add_assoc add_one_step add_step add_zero cancel_add zero_sum_split)
+export Addition.Derived (
+  add_assoc add_commutative add_one_step add_step add_substitutive add_zero cancel_add
+  zero_sum_split
+)
 end Addition
 
-export Addition (addOp step_add zero_add)
+export Addition (
+  add_assoc add_commutative add_one_step addOp add_step add_substitutive
+  add_zero cancel_add step_add zero_add zero_sum_split
+)
 
 end Natural
 end Lean4Axiomatic
