Lean4Axiomatic/Natural/Impl/Default/Order.lean
@@ -3,6 +3,8 @@ import Lean4Axiomatic.Natural.Order
 namespace Lean4Axiomatic
 namespace Natural
 
+namespace Default
+
 variable {ℕ : Type}
 variable [Core ℕ]
 variable [Addition.Base ℕ]
@@ -16,6 +18,8 @@ instance order_base : Order.Base ℕ where
 
   ltOp := inferInstance
   lt_defn {n m : ℕ} := Iff.intro id id
+
+end Default
 
 end Natural
 end Lean4Axiomatic
