Lean4Axiomatic/Natural/Order.lean
@@ -16,27 +16,40 @@ attribute [instance default+1] Order.Base.ltOp
 
 class Order.Derived (ℕ : Type) [Core ℕ] [Addition.Base ℕ]
     extends Order.Base ℕ where
-  le_subst_step : AA.Substitutive (α := ℕ) step (· ≤ ·) (· ≤ ·)
-  le_inject_step : AA.Injective (α := ℕ) step (· ≤ ·) (· ≤ ·)
-  le_subst_eqv : AA.Substitutive₂ (α := ℕ) (· ≤ ·) (· ≃ ·) (· → ·)
-  le_refl : Relation.Refl (α := ℕ) (· ≤ ·)
-  le_trans : Relation.Trans (α := ℕ) (· ≤ ·)
+  le_substitutive_step : AA.Substitutive (α := ℕ) step (· ≤ ·) (· ≤ ·)
+  le_injective_step : AA.Injective (α := ℕ) step (· ≤ ·) (· ≤ ·)
+  le_substitutive_eqv : AA.Substitutive₂ (α := ℕ) (· ≤ ·) (· ≃ ·) (· → ·)
+  le_reflexive : Relation.Refl (α := ℕ) (· ≤ ·)
+  le_transitive : Relation.Trans (α := ℕ) (· ≤ ·)
   le_antisymm {n m : ℕ} : n ≤ m → m ≤ n → n ≃ m
-  le_subst_add : AA.Substitutive₂ (α := ℕ) (· + ·) (· ≤ ·) (· ≤ ·)
-  le_cancel_add : AA.Cancellative₂ (α := ℕ) (· + ·) (· ≤ ·) (· ≤ ·)
+  le_substitutive_add : AA.Substitutive₂ (α := ℕ) (· + ·) (· ≤ ·) (· ≤ ·)
+  le_cancellative_add : AA.Cancellative₂ (α := ℕ) (· + ·) (· ≤ ·) (· ≤ ·)
   le_from_eqv {n m : ℕ} : n ≃ m → n ≤ m
   le_from_lt {n m : ℕ} : n < m → n ≤ m
   le_split {n m : ℕ} : n ≤ m → n < m ∨ n ≃ m
 
-  lt_subst_eqv : AA.Substitutive₂ (α := ℕ) (· < ·) (· ≃ ·) (· → ·)
-  lt_trans : Relation.Trans (α := ℕ) (· < ·)
+  lt_substitutive_eqv : AA.Substitutive₂ (α := ℕ) (· < ·) (· ≃ ·) (· → ·)
+  lt_transitive : Relation.Trans (α := ℕ) (· < ·)
   lt_zero {n : ℕ} : n ≮ 0
   lt_step {n : ℕ} : n < step n
   lt_step_le {n m : ℕ} : n < m ↔ step n ≤ m
   lt_split {n m : ℕ} : n < step m → n < m ∨ n ≃ m
   trichotomy {n m : ℕ} : AA.ExactlyOneOfThree (n < m) (n ≃ m) (n > m)
 
-attribute [instance] Order.Derived.le_subst_eqv
+attribute [instance] Order.Derived.le_substitutive_eqv
+
+namespace Order
+export Order.Base (le_defn leOp lt_defn ltOp)
+export Order.Derived (
+  le_antisymm le_reflexive le_split le_transitive
+  lt_split lt_step lt_step_le lt_zero trichotomy
+)
+end Order
+
+export Order (
+  le_antisymm le_defn le_reflexive le_split le_transitive leOp
+  lt_defn ltOp lt_split lt_step lt_step_le lt_zero trichotomy
+)
 
 end Natural
 end Lean4Axiomatic
